@prefix oceanmeta: <https://w3id.org/oceanmeta#> .
@prefix sosa: <http://www.w3.org/ns/sosa/> .
@prefix schema: <https://schema.org/> .
@prefix rdfs: <http://www.w3.org/2000/01/rdf-schema#> .
@prefix owl: <http://www.w3.org/2002/07/owl#> .
@prefix xsd: <http://www.w3.org/2001/XMLSchema#> .

#################################################################
#    Sensor Class
#################################################################

oceanmeta:Sensor a owl:Class ;
    rdfs:label "Sensor"@en ;
    rdfs:comment "A physical device capable of sensing or measuring an observable property. Subclass of sosa:Sensor."@en ;
    rdfs:subClassOf sosa:Sensor .

#################################################################
#    Properties
#################################################################

# Serial Number
oceanmeta:serialNumber a owl:DatatypeProperty ;
    rdfs:domain oceanmeta:Sensor ;
    rdfs:range xsd:string ;
    rdfs:label "Serial Number"@en ;
    rdfs:comment "Serial number of the sensor as provided by the manufacturer."@en ;
    rdfs:subPropertyOf schema:serialNumber .

# Sensor Model
oceanmeta:hasModel a owl:ObjectProperty ;
    rdfs:domain oceanmeta:Sensor ;
    rdfs:range oceanmeta:SensorModel ;
    rdfs:label "Sensor Model"@en ;
    rdfs:comment "The model or type of sensor, linking to a SensorModel resource."@en .
