@prefix goos: <https://www.ocean-ops.org/goosmeta#> .
@prefix schema: <https://schema.org/> .
@prefix rdfs: <http://www.w3.org/2000/01/rdf-schema#> .
@prefix owl: <http://www.w3.org/2002/07/owl#> .
@prefix xsd: <http://www.w3.org/2001/XMLSchema#> .
@prefix skos: <http://www.w3.org/2004/02/skos/core#> .

#################################################################
#    PlatformType Class
#################################################################

goos:PlatformType a owl:Class ;
    rdfs:label "Platform Type"@en ;
    rdfs:comment "A functional category of observation platforms such as Float, Wave Glider, or Tide Guage."@en ;
    rdfs:subClassOf schema:DefinedTerm .

#################################################################
#    Properties
#################################################################

# Unique PID
goos:id a owl:DatatypeProperty ;
    rdfs:label "Unique ID"@en ;
    rdfs:comment "A persistent, unique identifier (PID) for this platform type."@en ;
    rdfs:domain goos:PlatformType ;
    rdfs:range xsd:string .

goos:platformTypeName a owl:DatatypeProperty ;
    rdfs:domain goos:PlatformType ;
    rdfs:range xsd:string ;
    rdfs:subPropertyOf schema:name ;
    rdfs:label "Platform Type Name"@en ;
    rdfs:comment "Name of the platform type (e.g., Argo Float, Glider)."@en .

goos:platformTypeDescription a owl:DatatypeProperty ;
    rdfs:domain goos:PlatformType ;
    rdfs:range xsd:string ;
    rdfs:subPropertyOf schema:description ;
    rdfs:label "Platform Type Description"@en ;
    rdfs:comment "Description of the general characteristics or use of this platform type."@en .

goos:hasFamily a owl:ObjectProperty ;
    rdfs:domain goos:PlatformType ;
    rdfs:range goos:PlatformFamily ;
    rdfs:label "Has Platform Family"@en ;
    rdfs:comment "The broader platform family to which this type belongs (e.g., Subsurface Profiler, Moored Buoy or Fixed Station)."@en .