@prefix goos: <https://www.ocean-ops.org/goosmeta#> .
@prefix schema: <https://schema.org/> .
@prefix rdfs: <http://www.w3.org/2000/01/rdf-schema#> .
@prefix owl: <http://www.w3.org/2002/07/owl#> .
@prefix xsd: <http://www.w3.org/2001/XMLSchema#> .

#################################################################
#    SensorModel Class
#################################################################

goos:SensorModel a owl:Class ;
    rdfs:label "Sensor Model"@en ;
    rdfs:comment "A specification or model of a sensor, describing the types of variables it can observe. Subclass of schema:ProductModel."@en ;
    rdfs:subClassOf schema:ProductModel .

#################################################################
#    Properties
#################################################################

# Unique PID
goos:id a owl:DatatypeProperty ;
    rdfs:label "Unique ID"@en ;
    rdfs:comment "A persistent, unique identifier (PID) for this sensor model."@en ;
    rdfs:domain goos:SensorModel ;
    rdfs:range xsd:string .

# Sensor Model Name
goos:sensorModelName a owl:DatatypeProperty ;
    rdfs:subPropertyOf schema:name ;
    rdfs:domain goos:SensorModel ;
    rdfs:range xsd:string ;
    rdfs:label "Sensor Model Name"@en ;
    rdfs:comment "The commercial or technical name of the sensor model (e.g., Seabird SBE 37)."@en .

# Supported Variables
goos:supportsVariable a owl:ObjectProperty ;
    rdfs:domain goos:SensorModel ;
    rdfs:range goos:Variable ;
    rdfs:label "Supports Variable"@en ;
    rdfs:comment "A variable that this sensor model is capable of observing."@en .

goos:hasManufacturer a owl:ObjectProperty ;
    rdfs:label "Has Manufacturer"@en ;
    rdfs:comment "The organization that manufactures this sensor model."@en ;
    rdfs:domain goos:SensorModel ;
    rdfs:range goos:Organization ;
    rdfs:subPropertyOf schema:manufacturer .
