@prefix goos: <https://www.ocean-ops.org/goosmeta#> .
@prefix schema: <https://schema.org/> .
@prefix rdfs: <http://www.w3.org/2000/01/rdf-schema#> .
@prefix owl: <http://www.w3.org/2002/07/owl#> .
@prefix xsd: <http://www.w3.org/2001/XMLSchema#> .

#################################################################
#    WIGOS Program Class
#################################################################

goos:WIGOSProgram a owl:Class ;
    rdfs:label "WIGOS Program"@en ;
    rdfs:comment "A country-affiliated or institutional entity contributing to WIGOS through the execution of ocean observation missions and platform operations."@en ;
    rdfs:subClassOf schema:Organization .

#################################################################
#    Properties
#################################################################

# Unique PID
goos:id a owl:DatatypeProperty ;
    rdfs:label "Unique ID"@en ;
    rdfs:comment "A persistent, unique identifier (PID) for this WIGOS program."@en ;
    rdfs:domain goos:WIGOSProgram ;
    rdfs:range xsd:string .

goos:programName a owl:DatatypeProperty ;
    rdfs:label "Program Name"@en ;
    rdfs:subPropertyOf schema:name ;
    rdfs:domain goos:WIGOSProgram ;
    rdfs:range xsd:string .

goos:programDescription a owl:DatatypeProperty ;
    rdfs:label "Program Description"@en ;
    rdfs:subPropertyOf schema:description ;
    rdfs:domain goos:WIGOSProgram ;
    rdfs:range xsd:string .

goos:hasCountry a owl:ObjectProperty ;
    rdfs:label "Associated Country"@en ;
    rdfs:comment "The country to which this WIGOS Program is affiliated."@en ;
    rdfs:subPropertyOf schema:addressCountry ;
    rdfs:domain goos:WIGOSProgram ;
    rdfs:range goos:Country .

goos:hasOrganizationContribution a owl:ObjectProperty ;
    rdfs:label "Organization Contribution"@en ;
    rdfs:comment "A contribution made by an organization to this WIGOS Program, including its role and duration."@en ;
    rdfs:domain goos:WIGOSProgram ;
    rdfs:range goos:OrganizationContribution .
